imp_system/mem/MemIAproof.v
@@ -1,110 +1,8 @@
 From CRIS Require Import CRIS MemHeader MemA MemI ImpPrelude.
 From iris.algebra Require Import auth excl agree csum functions dfrac_agree.
 
-Local Open Scope nat_scope.
-
-Section AUX.
-  Context `{!crisG Γ Σ α β τ _S _I, !memG}.
-
-  Fixpoint is_list (ll: val) (xs: list val): iProp Σ :=
-    match xs with
-    | [] => (⌜ll = Vnullptr⌝)%I
-    | xhd :: xtl =>
-        (∃ lhd ltl, ⌜ll = Vptr (lhd, 0%Z)⌝ ∗ (lhd, 0%Z) |-> [xhd; ltl] ∗ is_list ltl xtl)%I
-    end.
-
-  Lemma unfold_is_list ll xs:
-    is_list ll xs =
-    match xs with
-    | [] => (⌜ll = Vnullptr⌝)%I
-    | xhd :: xtl =>
-      (∃ lhd ltl, ⌜ll = Vptr (lhd, 0%Z)⌝ ∗ (lhd, 0%Z) |-> [xhd; ltl] ∗ is_list ltl xtl)%I
-    end.
-  Proof using. destruct xs; ss. Qed.
-
-  Lemma unfold_is_list_cons ll xhd xtl:
-    is_list ll (xhd :: xtl) =
-    (∃ lhd ltl, ⌜ll = Vptr (lhd, 0%Z)⌝ ∗ (lhd, 0%Z) |-> [xhd; ltl] ∗ is_list ltl xtl)%I.
-  Proof using. eapply unfold_is_list. Qed.
-
-  Lemma is_list_wf ll xs:
-    (is_list ll xs) -∗ (⌜(ll = Vnullptr) ∨ (match ll with | Vptr (_, 0%Z) => True | _ => False end)⌝).
-  Proof using.
-    iIntros "L". destruct xs; ss; et.
-    { iPure "L" as L. iPureIntro. et. }
-    iDestruct "L" as (? ?) "(% & P & L)".
-    iPureIntro; right; subst; ss.
-  Qed.
-End AUX.
-
-Ltac Ztac := all_once_fast
-  ltac:(fun H =>
-    first[apply Z.leb_le in H|apply Z.ltb_lt in H|apply Z.leb_gt in H|apply Z.ltb_ge in H|idtac]).
-
-Section AUX2.
-  Lemma repeat_nth_some X (x: X) sz ofs (IN: ofs < sz) :
-    nth_error (repeat x sz) ofs = Some x.
-  Proof using.
-    ginduction sz; ii; ss.
-    - lia.
-    - destruct ofs; ss. exploit IHsz; et. lia.
-  Qed.
-
-  Lemma repeat_nth_none
-    X (x: X) sz ofs
-    (IN: ~(ofs < sz))
-    :
-    nth_error (repeat x sz) ofs = None
-    .
-  Proof using.
-    generalize dependent ofs. induction sz; ii; ss.
-    - destruct ofs; ss.
-    - destruct ofs; ss. { lia. } hexploit (IHsz ofs); et. lia.
-  Qed.
-
-  Lemma nth_error_empty
-    {X: Type} ofs
-    :
-    nth_error ([]: list X) ofs = None.
-  Proof using.
-    unfold nth_error. destruct ofs; ss.
-  Qed.
-
-  Lemma Z2nat_lt (x0: Z) (sz : nat)
-    (ZLT: (x0 < sz)%Z)
-    (SZ: (0 < sz))
-  :
-    (Z.to_nat x0 < sz).
-  Proof using.
-    induction sz.
-    - lia.
-    - induction x0.
-      * ss.
-      * ss.
-      assert (Z.succ sz = sz + 1)%Z. ss.
-      apply Z2Nat.inj_lt in ZLT; try lia.
-      * ss.
-  Qed.
-
-  Lemma Z_ne_le (z1 : Z) (z2 : Z)
-    (NE: z1 ≠ z2)
-    (LE: (z1 <=? z2)%Z)
-  :
-    (z1 < z2)%Z.
-  Proof using.
-    apply Z.leb_le in LE.
-    destruct (Z.eq_dec z1 z2) as [Heq | Hneq].
-  - (* Case: z1 = z2 (contradiction) *)
-    contradiction.
-  - (* Case: z1 ≠ z2 *)
-    lia.
-  Qed. (* Use NE and LE to conclude (z1 < z2)%Z *)
-
-End AUX2.
-
 Section RA.
-  Context `{_crisG: !crisG Γ Σ α β τ _S _I}.
-  Context `{_memG: !memG}.
+  Context `{!crisG Γ Σ α β τ _S _I, !memG}.
 
   Definition mem_wf (m : Mem.t) : Prop := ∀ b ofs v, m.(Mem.cnts) b ofs = Some v → b < m.(Mem.nb).
 
@@ -135,11 +33,11 @@ Section RA.
     ≡ (discrete_fun_singleton blk (discrete_fun_singleton ofs (Some (to_dfrac_agree q a)))).
   Proof using.
     intros b o; ss.
-    ss; case_bool_decide; des; simplify_eq; ss.
+    ss; case_bool_decide as H'; des; simplify_eq; ss.
     { destruct (decide (o = ofs)); subst; try nia.
       rewrite Z.sub_diag /= ?discrete_fun_lookup_singleton //.
     }
-    apply not_and_or in H; des; try by rewrite discrete_fun_lookup_singleton_ne //.
+    apply not_and_or in H'; des; try by rewrite discrete_fun_lookup_singleton_ne //.
     destruct (decide (b = blk)); subst;
       [rewrite discrete_fun_lookup_singleton discrete_fun_lookup_singleton_ne //; ii; clarify; nia
       |rewrite discrete_fun_lookup_singleton_ne //].
@@ -150,7 +48,7 @@ Section RA.
   Lemma points_to_transform blk ofs q l :
     own base_γ ((◯ _points_to_r (blk, ofs) (DfracOwn q) l): memRA)
     ⊢ [∗ list] i↦v ∈ l, (blk, (ofs + i)%Z) ↦{q} v.
-  Proof using _memG.
+  Proof using.
     gen ofs. induction l.
     - iIntros; eauto.
     - i. rewrite split_points_to_r. iIntros "[P L]".
@@ -159,8 +57,8 @@ Section RA.
       set (λ _ _, _). set (λ _ _, _).
       assert (y = y0).
       { extensionalities. subst y y0. ss.
-        replace (ofs + 1 + H)%Z with (ofs + S H)%Z by nia. refl. }
-      rewrite H. iFrame. unfold mem_points_to_singleton, mem_points_to_singleton_r; ss.
+        replace (ofs + 1 + H0)%Z with (ofs + S H0)%Z by nia. refl. }
+      rewrite H0. iFrame. unfold mem_points_to_singleton, mem_points_to_singleton_r; ss.
       rewrite Z.add_0_r. iFrame.
   Qed.
 
@@ -173,10 +71,10 @@ Section RA.
     specialize (EQ0 0). rr in EQ0. des.
     edestruct EQ0; s; eauto using elem_of_list.
     des. ss. destruct (agree_car f.2) eqn: E.
-    - rewrite E in H. rr in H. inv H.
-    - exists l. f_equal. rr in H0. depdes H0. rewrite E in EQ1.
+    - rewrite E in H0. rr in H0. inv H0.
+    - exists l. f_equal. rr in H1. depdes H1. rewrite E in EQ1.
       edestruct (EQ1 o); eauto using elem_of_list. des.
-      rr in H1. depdes H1. rr in H0. depdes H0; ss. rr in H0. depdes H0.
+      rr in H2. depdes H2. rr in H1. depdes H1; ss. rr in H1. depdes H1.
   Qed.
 
   Lemma to_frac_full_valid_inv A c (v: leibnizO A)
@@ -195,21 +93,21 @@ Section RA.
     :
     own γ ((● mem_src): memRA)
     ⊢ |==>
-    own γ ((● (mem_src ⋅ _points_to_r (blk, 0%Z) (DfracOwn 1) (repeat Vundef sz))): memRA)
-    ∗ own γ ((◯ _points_to_r (blk, 0%Z) (DfracOwn 1) (repeat Vundef sz)): memRA).
-  Proof using _memG.
+    own γ ((● (mem_src ⋅ _points_to_r (blk, 0%Z) (DfracOwn 1) (replicate sz Vundef))): memRA)
+    ∗ own γ ((◯ _points_to_r (blk, 0%Z) (DfracOwn 1) (replicate sz Vundef)): memRA).
+  Proof using.
     iIntros "P". rewrite -own_op.
     iApply (own_update with "P"). apply auth_update_alloc.
-    apply local_update_discrete. i. rewrite H0.
+    apply local_update_discrete. i. rewrite H1.
     split; cycle 1.
     - destruct mz; simpl opM in *.
       + rewrite left_id (comm _ c). et.
       + rewrite left_id. et.
-    - rewrite -H0. ii. rewrite !discrete_fun_lookup_op /_points_to_r.
+    - rewrite -H1. ii. rewrite !discrete_fun_lookup_op /_points_to_r.
       case_bool_decide; s; cycle 1.
-      { rewrite right_id. apply H. }
-      hexploit (SIM blk x0). i; subst; des; rewrite H1; clarify.
-      + rewrite H2; case_match; ss.
+      { rewrite right_id. apply H0. }
+      hexploit (SIM blk x0). i; subst; des; rewrite H2; clarify.
+      + rewrite H3; case_match; ss.
       + exploit WF; et. nia.
   Qed.
 
@@ -226,12 +124,12 @@ Section RA.
     dup WF. rewrite auth_both_valid_discrete in WF. ss. des.
     unfold included in *. des. specialize (WF b ofs). iris_tac.
     rewrite ->!discrete_fun_lookup_singleton in *.
-    destruct (SIM b ofs); des; rewrite H in WF.
+    destruct (SIM b ofs); des; rewrite H0 in WF.
     { destruct (z b ofs); ss; rewrite -?Some_op ?right_id in WF; inv WF. }
     rewrite -WF. destruct (z b ofs); rr in WF; depdes WF.
-    - assert (EXT: to_dfrac_agree (DfracOwn q) v ≼ to_dfrac_agree (DfracOwn 1) v0) by (rewrite H1; et).
+    - assert (EXT: to_dfrac_agree (DfracOwn q) v ≼ to_dfrac_agree (DfracOwn 1) v0) by (rewrite H2; et).
       eapply dfrac_agree_included in EXT. des; subst. rr in EXT0. subst. et.
-    - eapply to_frac_agree_inv in H1. ss. des. depdes H2. et.
+    - eapply to_frac_agree_inv in H2. ss. des. depdes H3. et.
   Qed.
 
   Lemma mem_ra_update v_new v (mem_s: _memRA) mem_t b ofs :
@@ -241,14 +139,14 @@ Section RA.
       (b, ofs) ↦{1} v_new.
   Proof using.
     iIntros "%SIM [Auth Frag]".
-    iPoseProof ((mem_ra_lookup _ _ _ _ _ _ SIM) with "[Auth Frag]") as "[%H %_]"; iFrame.
+    iPoseProof ((mem_ra_lookup _ _ _ _ _ _ SIM) with "[Auth Frag]") as "[%H' %_]"; iFrame.
     rewrite -own_op.
     iApply (own_update_2 with "Auth Frag").
     rewrite /mem_points_to_singleton_r /= auth_update //; apply discrete_fun_local_update.
     intros b2; apply discrete_fun_local_update; intros o2.
     destruct (decide (b2 = b)); subst.
     { destruct (decide (o2 = ofs)); subst.
-      { rewrite H ?discrete_fun_lookup_singleton /mem_ra_upd; case_bool_decide; [|naive_solver].
+      { rewrite H' ?discrete_fun_lookup_singleton /mem_ra_upd; case_bool_decide; [|naive_solver].
         apply option_local_update, exclusive_local_update; ss.
       }
       rewrite ?discrete_fun_lookup_singleton /mem_ra_upd; case_bool_decide; [naive_solver|].
@@ -263,7 +161,7 @@ Section RA.
     mem_wf mem_t →
     own base_γ (● mem_s) ∗ (b, ofs) ↦{1} v ⊢
     |==> own base_γ (● mem_ra_upd mem_s b ofs None).
-  Proof using _memG.
+  Proof using.
     iIntros "% % [Auth Frag]".
     iApply (own_update_2 with "Auth Frag").
     rewrite /mem_points_to_singleton_r auth_update_dealloc //=.
@@ -293,23 +191,22 @@ Section RA.
     - des_ifs.
     - iPoseProof (mem_ra_lookup with "[B P2]") as "%"; et; iFrame.
       specialize (SIM n0 z). des; subst; ss.
-      + rewrite SIM in H. r in H. depdes H.
+      + rewrite SIM in H0. r in H0. depdes H0.
       + rewrite SIM0. iPureIntro. des_ifs.
     - destruct n; ss.
     - iPoseProof (mem_ra_lookup with "[B P1]") as "%"; et; iFrame.
       specialize (SIM n0 z). des; subst; ss.
-      + rewrite SIM in H. rr in H. depdes H.
+      + rewrite SIM in H0. rr in H0. depdes H0.
       + rewrite SIM0. iPureIntro. des_ifs.
     - iPoseProof (mem_ra_lookup with "[B P1]") as "%"; et; iFrame.
       iPoseProof (mem_ra_lookup with "[B P2]") as "%"; et; iFrame.
       dup SIM. specialize (SIM n z). des; subst; ss.
-      { rewrite SIM in H. rr in H. depdes H. }
+      { rewrite SIM in H0. rr in H0. depdes H0. }
       specialize (SIM0 n0 z0). des; subst; ss.
-      { rewrite SIM0 in H0. rr in H0. depdes H0. }
+      { rewrite SIM0 in H1. rr in H1. depdes H1. }
       rewrite SIM1 SIM2. s.
       repeat case_bool_decide; ss; des; simplify_eq.
   Qed.
-
 End RA.
 
 Module MemIA. Section MemIA.
@@ -343,737 +240,11 @@ Module MemIA. Section MemIA.
     rewrite H2. et.
   Qed.
 
-  Ltac init_simF :=
-    rewrite /ISim.sim_fun; simplify_map_eq; intros ??; eexists; split; first refl;
-    iIntros (arg st_src st_tgt) "IST"; iApply wsim_isim;
-    rewrite /SB.sandbox_body /=.
-    (* /SModTr.trans_fnsem /=. *)
   Local Definition state : Type := gmap key (option Any.t).
   Local Definition post (R_s R_t : Type) : Type := state * R_s → state * R_t → iProp Σ.
 
   Local Definition rel : Type := ∀ R_s R_t : Type,
     post R_s R_t → bool → bool → state * itree crisE R_s → state * itree crisE R_t → iProp Σ.
-
-  (* TEMP *)
-  Ltac simplify_msk msk :=
-    (* try match goal with
-    | H :  context [msk _ _ = _] |- _ => rewrite H
-    end; *)
-    lazymatch goal with
-    | [ |- match ?P with true => _ | false => _ end] =>
-        let r := eval vm_compute in P in
-        change P with r in *
-    end.
-
-
-Tactic Notation "red_bind" tactic(tac) :=
-  lazymatch goal with
-  | [ |- @ITree.bind _ _ _ ?itr _ = _ ] =>
-      lazymatch itr with
-      | Ret _ => etransitivity; [ eapply bind_ret_l | s; tac ]
-      | Tau _ => eapply bind_tau
-      | vis _ _ => eapply vis_bind
-      | assumeK _ _ => eapply assumeK_bind
-      | guaranteeK _ _ => eapply guaranteeK_bind
-      | unwrapUK _ _ => eapply unwrapUK_bind
-      | unwrapNK _ _ => eapply unwrapNK_bind
-      | RealUpdateK _ _ _ => eapply RealUpdateK_bind
-      (* | SBRed.putSB _ _ _ _ _ _ => eapply SBRed.putSB_bind
-      | SBRed.getSB _ _ _ _ _ => eapply SBRed.getSB_bind
-      | SBRed.callSB _ _ _ _ _ _ => eapply SBRed.callSB_bind
-      | SBRed.spawnSB _ _ _ _ _ _ => eapply SBRed.spawnSB_bind *)
-      | @ITree.bind _ _ _ _ _ => eapply bind_bind
-      | _ => reflexivity
-      end
-  end.
-
-Tactic Notation "red_SB" tactic(tac) :=
-  lazymatch goal with
-  | [ |- @SB.sandbox ?Σ ?msk ?R ?itr = _ ] =>
-      lazymatch itr with
-      | Ret _ =>
-          eapply SBRed.ret
-      | Tau _ =>
-          eapply SBRed.tau
-      | vis _ ?k =>
-          etransitivity; [eapply SBRed.vis | s; tac ]
-      (* | assumeK _ _ =>
-          eapply SBRed.assumeK *)
-      (* | guaranteeK _ _ =>
-          eapply SBRed.guaranteeK *)
-      (* | unwrapUK _ _ =>
-          eapply SBRed.unwrapUK *)
-      (* | unwrapNK _ _ =>
-          eapply SBRed.unwrapNK *)
-      (* | RealUpdateK _ _ _ =>
-          eapply SBRed.ruK *)
-      | @ITree.bind _ _ _ _ _ =>
-          eapply SBRed.bind
-      | _ =>
-          reflexivity
-      end
-  end.
-
-(* Ltac unfold_sp_exact sp name :=
-  try match goal with
-      [ H : sp_incl _ sp |- _ ] =>
-        let RW := fresh "_RW" in
-        let ND := fresh "_ND" in
-        edestruct H as [ND RW];
-        erewrite (RW name);
-        [| revert ND; unfold to_sp;
-           match goal with [|-context[alist_find _ ?x]] => rewrite /x end;
-           unseal CRIS; i;
-           alist_find_simpl;
-           refl];
-        simpl unwrapN; clear ND RW
-    end. *)
-
-Tactic Notation "red_S" tactic(tac) :=
-  lazymatch goal with
-  | [ |- @SModTr.trans ?Γ ?Σ ?α ?β ?τ ?_S ?_I ?_crisG ?concG ?sp ?N ?stid ?R ?itr = _ ] =>
-      lazymatch itr with
-      | Ret _ =>
-          eapply SRed.ret
-      | Tau _ =>
-          eapply SRed.tau
-      | vis (Assume _) _ =>
-          eapply SRed.vis_agE
-      | vis (AssumeRes _) _ =>
-          eapply SRed.vis_agE
-      | vis (Guarantee _) _ =>
-          eapply SRed.vis_agE
-      | vis (Spawn ?fn _) _ =>
-          etransitivity;
-          [ eapply SRed.vis_spawn
-          | unfold SModTr.HoareSpawn;
-            tac
-          ]
-      | vis (Yield _) _ =>
-          etransitivity;
-          [ eapply SRed.vis_yield
-          | tac
-          ]
-      | vis GetTid _ =>
-          etransitivity;
-          [ eapply SRed.vis_gettid
-          | tac
-          ]
-      | vis (Call ?fn _) _ =>
-          etransitivity;
-          [ eapply SRed.vis_call
-          | unfold SModTr.HoareCall;
-            tac
-          ]
-      | vis (SPut _ _) _ =>
-          eapply SRed.vis_pgE
-      | vis (SGet _) _ =>
-          eapply SRed.vis_pgE
-      | vis (Choose _) _ =>
-          eapply SRed.vis_coreE
-      | vis (Take _) _ =>
-          eapply SRed.vis_coreE
-      | vis (IO _ _) _ =>
-          eapply SRed.vis_coreE
-      (* | assumeK _ _ =>
-          eapply SRed.assumeK
-      | guaranteeK _ _ =>
-          eapply SRed.guaranteeK
-      | unwrapUK _ _ =>
-          eapply SRed.unwrapUK
-      | unwrapNK _ _ =>
-          eapply SRed.unwrapNK *)
-      (* | RealUpdateK _ _ _ =>
-          eapply SRed.ruK *)
-      | @ITree.bind _ _ _ _ _ =>
-          eapply SRed.bind
-      | _ =>
-          reflexivity
-      end
-  end.
-
-Ltac _hnorm_itr :=
-  lazymatch goal with
-  | |- match bool_decide ?P with | true => ?A | false => ?B end = _ =>
-      tryif is_closed_term P
-      then
-        let r := eval vm_compute in (bool_decide P) in
-        change (bool_decide P) with r in *;
-        s; _hnorm_itr
-      else reflexivity
-  | [ |- Ret _ = _ ] =>
-      reflexivity
-  | [ |- Tau _ = _ ] =>
-      reflexivity
-  | [ |- vis _ _ = _ ] =>
-      reflexivity
-  | [ |- @ITree.bind ?E ?T ?U ?itr ?ktr = _ ] =>
-      etransitivity;
-      [ let itr' := fresh "itr" in
-        cong (fun (itr' : itree E T) => @ITree.bind E T U itr' ktr); _hnorm_itr
-      | red_bind (do 1 _hnorm_itr) ]
-  (* | [ |- @SB.sandbox ?Σ ?R ?img ?imports ?scopes ?itr = _ ] =>
-      etransitivity;
-      [ cong (@SB.sandbox Σ R img imports scopes); _hnorm_itr | red_SB ] *)
-  | [ |- @SB.sandbox ?Σ ?msk ?R ?itr = _ ] =>
-      etransitivity;
-      [ cong (@SB.sandbox Σ msk R); _hnorm_itr | red_SB (do 1 _hnorm_itr) ]
-  (* | [ |- @SModTr.trans ?Γ ?Σ ?α ?β ?τ ?_S ?_I ?_crisG ?concG ?img ?sp ?R ?itr = _ ] =>
-      etransitivity;
-      [ cong (@SModTr.trans Γ Σ α β τ _S _I _crisG concG img sp R); _hnorm_itr
-      | red_S (do 1 _hnorm_itr) ] *)
-  | [ |- @SModTr.trans ?Γ ?Σ ?α ?β ?τ ?_S ?_I ?_crisG ?concG ?sp ?N ?stid ?R ?itr = _ ] =>
-      etransitivity;
-      [ cong (@SModTr.trans Γ Σ α β τ _S _I _crisG concG sp N stid R); _hnorm_itr
-      | red_S (do 1 _hnorm_itr) ]
-  | [ |- trigger _ = _ ] =>
-      eapply trigger_vis
-  (* | [ |- assume _ = _ ] =>
-      eapply assume_assumeK
-  | [ |- guarantee _ = _ ] =>
-      eapply guarantee_guaranteeK *)
-  (* | [ |- unwrapU _ = _ ] =>
-      eapply unwrapU_unwrapUK
-  | [ |- unwrapN _ = _ ] =>
-      eapply unwrapN_unwrapNK *)
-  | [ |- RealUpdate _ _ = _ ] =>
-      eapply RealUpdate_RealUpdateK
-  | [ |- SModTr.HoareCall _ _ _ = _ ] =>
-      unfold SModTr.HoareCall;
-      _hnorm_itr
-  | [ |- fbody_trivial _ = _ ] =>
-      unfold fbody_trivial;
-      _hnorm_itr
-  | [ |- cput _ _ = _ ] =>
-      unfold cput;
-      _hnorm_itr
-  | [ |- cgetU _ = _ ] =>
-      unfold cgetU;
-      _hnorm_itr
-  | [ |- cgetN _ = _ ] =>
-      unfold cgetN;
-      _hnorm_itr
-  | [ |- cfunU _ _ = _ ] =>
-      unfold cfunU;
-      _hnorm_itr
-  | [ |- cfunN _ _ = _ ] =>
-      unfold cfunN;
-      _hnorm_itr
-  | [ |- ccallU _ _ = _ ] =>
-      unfold ccallU;
-      _hnorm_itr
-  | [ |- ccallN _ _ = _ ] =>
-      unfold ccallN;
-      _hnorm_itr
-  | [ |- triggerUB = _ ] =>
-      unfold triggerUB;
-      _hnorm_itr
-  | [ |- triggerNB = _ ] =>
-      unfold triggerNB;
-      _hnorm_itr
-  | [ |- ?itr = _ ] =>
-      reflexivity
-  end.
-
-Ltac hnorm_itr :=
-  etransitivity;
-  [ _hnorm_itr
-  | s;
-    lazymatch goal with
-    | |- Ret _ = _ =>
-        reflexivity
-    | |- Tau _ = _ =>
-        reflexivity
-    | |- vis _ _ = _ =>
-        rewrite ?resum_to_subevent ?subevent_subevent;
-        eapply vis_trigger
-    | |- assumeK _ _ = _ =>
-        eapply assumeK_assume
-    | |- guaranteeK _ _ = _ =>
-        eapply guaranteeK_guarantee
-    | |- unwrapUK _ _ = _ =>
-        eapply unwrapUK_unwrapU
-    | |- unwrapNK _ _ = _ =>
-        eapply unwrapNK_unwrapN
-    | |- RealUpdateK _ _ _ = _ =>
-        eapply RealUpdateK_RealUpdate
-    (* | [ |- SBRed.putSB _ _ _ _ _ _ = _ ] =>
-        eapply SBRed.putSB_SPut *)
-    (* | [ |- SBRed.getSB _ _ _ _ _ = _ ] =>
-        eapply SBRed.getSB_SGet *)
-    (* | [ |- SBRed.callSB _ _ _ _ _ _ = _ ] =>
-        eapply SBRed.callSB_Call *)
-    (* | [ |- SBRed.spawnSB _ _ _ _ _ _ = _ ] =>
-        eapply SBRed.spawnSB_Spawn *)
-    | [ |- _ = _ ] =>
-        reflexivity
-    end
-  ].
-Ltac replace_l :=
-  lazymatch goal with
-  | [ |- environments.envs_entails ?env (?rel (?st_src, ?itr_src) (?st_tgt, ?itr_tgt)) ] =>
-      refine (eq_ind_r (fun itr_src' => environments.envs_entails env (rel (st_src, itr_src') (st_tgt, itr_tgt))) _ _); cycle 1
-  end.
-
-Ltac replace_r :=
-  lazymatch goal with
-  | [ |- environments.envs_entails ?env (?rel (?st_src, ?itr_src) (?st_tgt, ?itr_tgt)) ] =>
-      refine (eq_ind_r (fun itr_tgt' => environments.envs_entails env (rel (st_src, itr_src) (st_tgt, itr_tgt'))) _ _); cycle 1
-  end.
-
-Ltac norm_l := replace_l; [s; hnorm_itr|].
-Ltac norm_r := replace_r; [s; hnorm_itr|].
-
-Tactic Notation "norm_l" "with" tactic(tac) :=
-  let marker := fresh "MARKER" in
-  set_marker marker;
-  hide_ihyps;
-  norm_l;
-  tac;
-  show_until marker.
-
-Tactic Notation "norm_r" "with" tactic(tac) :=
-  let marker := fresh "MARKER" in
-  set_marker marker;
-  hide_ihyps;
-  norm_r;
-  tac;
-  show_until marker.
-
-Tactic Notation "norm" "with" tactic(tac) :=
-  let marker := fresh "MARKER" in
-  set_marker marker;
-  hide_ihyps;
-  norm_l;
-  norm_r;
-  tac;
-  show_until marker.
-
-  (* TODO : improve *)
-  Ltac prove_inline_cond :=
-    simplify_map_eq; ss.
-
-  Tactic Notation "iwcase" tactic(itac) tactic(wtac) :=
-    match goal with
-    | [ |- environments.envs_entails _ (isim _ _ _ _ _ _ _ _ _ _ _) ] => itac
-    | [ |- environments.envs_entails _ (wsim _ _ _ _ _ _ _ _ _ _ _ _ _) ] => wtac
-    end.
-
-  Lemma map_Forall_union_with `{Countable K} {V} (m1 m2 : gmap K (option V)) :
-    map_Forall (const is_Some) (union_with (λ _ _, Some None) m1 m2) →
-    map_Forall (const is_Some) m1 ∧ map_Forall (const is_Some) m2.
-  Proof.
-    rewrite ?map_Forall_lookup => Hwf; split; intros i v Hi; move: (Hwf i v);
-      rewrite lookup_union_with Hi; repeat destruct (_ !! i) as [[|]|]; ss; clarify; eauto.
-  Qed.
-
-  Lemma lookup_union_with_l `{Countable K} {V} (m1 m2 : gmap K (option V)) (k : K) (v : V):
-    map_Forall (const is_Some) (union_with (λ _ _, Some None) m1 m2) →
-    m1 !! k = Some (Some v) →
-    union_with (λ _ _, Some None) m1 m2 !! k = Some (Some v).
-  Proof.
-    intros Hwf Hm1; rewrite lookup_union_with Hm1; destruct (m2 !! k) as [[|]|] eqn : Hm2; ss;
-      apply map_Forall_lookup in Hwf; move: (Hwf k None); rewrite lookup_union_with Hm1 Hm2;
-      move => /(_ eq_refl) [? ?] //.
-  Qed.
-
-  Lemma lookup_union_with_r `{Countable K} {V} (m1 m2 : gmap K (option V)) (k : K) (v : V):
-    map_Forall (const is_Some) (union_with (λ _ _, Some None) m1 m2) →
-    m2 !! k = Some (Some v) →
-    union_with (λ _ _, Some None) m1 m2 !! k = Some (Some v).
-  Proof.
-    intros Hwf Hm2; rewrite lookup_union_with Hm2; destruct (m1 !! k) as [[|]|] eqn : Hm1; ss;
-      apply map_Forall_lookup in Hwf; move: (Hwf k None); rewrite lookup_union_with Hm1 Hm2;
-      move => /(_ eq_refl) [? ?] //.
-  Qed.
-
-  Lemma insert_union_with_l `{Countable K} {V} (m1 m2 : gmap K (option V)) (k : K) v :
-    map_Forall (const is_Some) (union_with (λ _ _, Some None) m1 m2) →
-    is_Some (m1 !! k) →
-    <[k := v]> (union_with (λ _ _, Some None) m1 m2) =
-    union_with (λ _ _, Some None) (<[k := v]> m1) m2.
-  Proof.
-    intros Hwf [? Hm1]; apply insert_union_with_l.
-    destruct (m2 !! k) as [[|]|] eqn : Hm2; ss;
-      apply map_Forall_lookup in Hwf; move: (Hwf k None); rewrite lookup_union_with Hm1 Hm2;
-      move => /(_ eq_refl) [? ?] //.
-  Qed.
-
-  Lemma insert_union_with_r `{Countable K} {V} (m1 m2 : gmap K (option V)) (k : K) v :
-    map_Forall (const is_Some) (union_with (λ _ _, Some None) m1 m2) →
-    is_Some (m2 !! k) →
-    <[k := v]> (union_with (λ _ _, Some None) m1 m2) =
-    union_with (λ _ _, Some None) m1 (<[k := v]> m2).
-  Proof.
-    intros Hwf [? Hm2]; apply insert_union_with_r.
-    destruct (m1 !! k) as [[|]|] eqn : Hm1; ss;
-      apply map_Forall_lookup in Hwf; move: (Hwf k None); rewrite lookup_union_with Hm1 Hm2;
-      move => /(_ eq_refl) [? ?] //.
-  Qed.
-
-Ltac is_key_in k m :=
-  match m with
-  | {[ k := _ ]} => idtac
-  | <[ k := _ ]> _ => idtac
-  | <[ _ := _ ]> ?rest => is_key_in k rest
-  | union_with _ ?l ?r => first [ is_key_in k l | is_key_in k r ]
-  | _ => fail "Key not syntactically found"
-  end.
-
-Ltac solve_map_lookup_symbolic NODT :=
-  match goal with
-  | [ |- union_with ?f ?l ?r !! ?k = _ ] =>
-      tryif is_key_in k l 
-      then (
-        eapply lookup_union_with_l;
-        [eauto|eapply map_Forall_union_with in NODT as [NODT _]];
-        solve_map_lookup_symbolic NODT
-      )
-      else (
-        eapply lookup_union_with_r;
-        [eauto|eapply map_Forall_union_with in NODT as [_ NODT]];
-        solve_map_lookup_symbolic NODT
-      )
-  | [ |- <[ ?k' := ?v ]> ?m !! ?k = _ ] =>
-      (* Case: Insert *)
-      tryif unify k' k
-      then (rewrite lookup_insert; reflexivity)
-      else (
-        rewrite lookup_insert_ne; [|let Hc := fresh "" in intro Hc; inversion Hc; done];
-        solve_map_lookup_symbolic NODT
-      )
-  | [ |- {[ ?k' := ?v ]} !! ?k = _ ] =>
-      (* Case: Singleton *)
-      unify k' k; apply lookup_singleton
-  | |- ?A => 
-      (* idtac "Leaf reached or structure unknown";  *) fail
-  end.
-
-Ltac state_lookup_simpl NOD :=
-  let GOAL := fresh "GOAL" in
-  set (a := _ !! _); pattern a; subst a;
-  match goal with [|- ?G _] => set (GOAL := G) end;
-  eapply (eq_ind_r GOAL); [|solve_map_lookup_symbolic NOD];
-  rewrite /GOAL /=; clear GOAL.
-
-(* TODO : the complexity of this tactic is terrible - make it better *)
-Ltac state_insert_simpl NODT :=
-  let GOAL := fresh "GOAL" in
-  set (a := <[_:=_]> _); pattern a; subst a;
-  match goal with [|- ?G _] => set (GOAL := G) end;
-  eapply (eq_ind_r GOAL);
-  [|
-    match goal with
-    | [ |- <[?k:=?v]> (union_with ?f ?l ?r) = _ ] =>
-        tryif is_key_in k l
-        then (
-          etransitivity;
-          [ eapply insert_union_with_l;
-            [ eauto
-            | eapply map_Forall_union_with in NODT as [NODT _];
-              eexists; state_lookup_simpl NODT; reflexivity
-            ]
-          | eapply map_Forall_union_with in NODT as [NODT _]; 
-            state_insert_simpl NODT ]
-        )
-        else (
-          etransitivity;
-          [ eapply insert_union_with_r;
-            [ eauto
-            | eapply map_Forall_union_with in NODT as [_ NODT];
-              eexists; state_lookup_simpl NODT; reflexivity
-            ]
-          | eapply map_Forall_union_with in NODT as [_ NODT]; 
-            state_insert_simpl NODT ]
-        )
-    | [ |- <[?k:=_]>{[?k':=?v]} = _ ] => (* Case: Singleton *)
-        unify k' k; apply insert_singleton
-    | [ |- <[?k:=_]>(<[?k':=?v]>?m) = _ ] => (* Case: Insert *)
-        tryif unify k' k
-        then (rewrite insert_insert; reflexivity)
-        else (
-          rewrite insert_ne; [|let Hc := fresh "" in intro Hc; inversion Hc; done];
-          state_insert_simpl NODT
-        )
-    
-    | |- ?A => 
-        (* idtac "Leaf reached or structure unknown";  *) fail
-    end
-  ];
-  rewrite /GOAL //=; clear GOAL.
-
-(* Ltac state_insert_simpl NOD :=
-  let GOAL := fresh "GOAL" in
-  set (a := <[_:=_]> _); pattern a; subst a;
-  match goal with [|- ?G _] => set (GOAL := G) end;
-  eapply (eq_ind_r GOAL); [|solve_map_insert_symbolic NOD];
-  rewrite /GOAL /=; clear GOAL. *)
-
-Ltac _wstep_l :=
-  match goal with
-  | [ |- environments.envs_entails _ (wsim _ _ _ _ _ _ _ _ _ _ _ (_, tau;; _) _) ] =>
-      iApply wsim_tau_src
-  | [ |- environments.envs_entails _ (wsim _ _ _ _ _ _ _ _ _ _ _ (_, Ret _ >>= _) _) ] =>
-      rewrite bind_ret_l
-  | [ |- environments.envs_entails _ (wsim _ _ _ _ _ _ _ _ _ _ _ (_, trigger (Take _) >>= _) _) ] =>
-      let name := fresh "_q" in iApply wsim_take_src; iIntros (name)
-  | [ |- environments.envs_entails _ (wsim _ _ _ _ _ _ _ _ _ _ _ (_, trigger (Assume ?P) >>= _) _) ] =>
-      unfold_pre_post_term P; iApply wsim_assume_src; iIntrosFresh "ASM"
-      (* first [
-        tcsearch constr:(WP P)
-          ltac:(fun c =>
-            iApply (wsim_assume_src_WP _ _ _ _ _ _ _ _ _ _ _ _ _ _ _ (i:=c)); simpl);
-        match goal with
-        | [ |- environments.envs_entails _ (?P' -∗ _)] =>
-          unfold_pre_post_term P'; iIntrosFresh "ASM"
-        end
-      | unfold_pre_post_term P; iApply wsim_assume_src; iIntrosFresh "ASM"
-      ] *)
-  | [ |- environments.envs_entails _ (wsim _ _ _ _ _ _ _ _ _ _ _ (_, trigger (AssumeRes _) >>= _) _) ] =>
-      iApply wsim_assume_res_src; iIntrosFresh "ASM"
-  | [ |- environments.envs_entails _ (wsim _ _ _ _ _ _ _ _ _ _ _ (_, assume _ >>= _) _) ] =>
-      let name := fresh "asm" in iApply wsim_asm_src; iIntros (name)
-  (* | [ |- environments.envs_entails _ (wsim _ _ _ _ _ _ _ _ _ _ _ (_, (SB.sandbox _ _ _ (trigger (SPut _ _))) >>= _) _) ] =>
-      iApply wsim_nodup_src; iIntros (?); iApply wsim_sput_src_sandbox; [s;eauto|alist_upd_simpl]
-  | [ |- environments.envs_entails _ (wsim _ _ _ _ _ _ _ _ _ _ _ (_, (SB.sandbox _ _ _ (trigger (SGet _))) >>= _) _) ] =>
-      let name := fresh "NODS" in
-      iApply wsim_nodup_src; iIntros (name); iApply wsim_sget_src_sandbox; [s;eauto|alist_find_simpl]; clear name *)
-  | [ |- environments.envs_entails _ (wsim _ _ _ _ _ _ _ _ _ _ _ (_, unwrapU ?ox >>= _) _) ] =>
-      let name := fresh "_q" in
-      iApply wsim_unwrapU_src; iIntros (name) "%";
-      match goal with [ H: ?x = Some _ |- _ ] => let G := fresh "G" in rename H into G; try rewrite -> G in * end
-  end.
-
-Ltac wstep_l_core :=
-  _wstep_l; try alist_find_simpl; s; des_pairs; s.
-
-Ltac wstep_l :=
-  norm_l with do 1 try wstep_l_core.
-
-Ltac wsteps_l :=
-  let marker := fresh "MARKER" in
-  set_marker marker;
-  hide_ihyps;
-  norm_l;
-  (hrepeat (do 1 wstep_l_core; norm_l));
-  show_until marker.
-
-Ltac _wstep_r :=
-  match goal with
-  (** tgt **)
-  | [ |- environments.envs_entails _ (wsim _ _ _ _ _ _ _ _ _ _ _ _ (_, tau;; _)) ] =>
-      iApply wsim_tau_tgt
-  | [ |- environments.envs_entails _ (wsim _ _ _ _ _ _ _ _ _ _ _ _ (_, Ret _ >>= _) ) ] =>
-      rewrite bind_ret_l
-  | [ |- environments.envs_entails _ (wsim _ _ _ _ _ _ _ _ _ _ _ _ (_, trigger (Choose _) >>= _) ) ] =>
-      let name := fresh "_q" in iApply wsim_choose_tgt; iIntros (name)
-  | [ |- environments.envs_entails _ (wsim _ _ _ _ _ _ _ _ _ _ _ _ (_, trigger (Guarantee ?P) >>= _) ) ] =>
-      unfold_pre_post_term P; iApply wsim_guarantee_tgt; iIntrosFresh "GRT"
-  | [ |- environments.envs_entails _ (wsim _ _ _ _ _ _ _ _ _ _ _ _ (_, guarantee _ >>= _)) ] =>
-      let name := fresh "grt" in iApply wsim_guar_tgt; iIntros (name)
-  | [ |- environments.envs_entails _ (wsim _ _ _ _ _ _ _ _ _ _ _ _ (_, trigger (SGet _) >>= _)) ] =>
-      let NODT := fresh "NODT" in
-      iApply wsim_nodup_tgt; iIntros (NODT);
-      iApply wsim_sget_tgt; state_lookup_simpl NODT; clear NODT
-  | [ |- environments.envs_entails _ (wsim _ _ _ _ _ _ _ _ _ _ _ _ (_, trigger (SPut _ _) >>= _)) ] =>
-      let NODT := fresh "NODT" in
-      iApply wsim_nodup_tgt; iIntros (NODT);
-      iApply wsim_sput_tgt; state_insert_simpl NODT; clear NODT
-  end.
-
-Ltac wstep_r_core :=
-  _wstep_r; s; des_pairs; s.
-
-Ltac wstep_r :=
-  norm_r with do 1 try wstep_r_core.
-
-Ltac wsteps_r :=
-  let marker := fresh "MARKER" in
-  set_marker marker;
-  hide_ihyps;
-  norm_r;
-  (hrepeat (do 1 wstep_r_core; norm_r));
-  show_until marker.
-
-Ltac _wstep :=
-  match goal with
-  | [ |- environments.envs_entails _ (wsim _ _ _ _ _ _ _ _ _ _ _ (_, Ret _) (_, Ret _))] =>
-      iApply wsim_unfold; iIntros "?"; iApply wsim_ret; iFrame
-  | [ |- environments.envs_entails _ (wsim _ _ _ _ _ _ _ _ _ _ _ (_, trigger (IO _ _) >>= _) (_, trigger (IO _ _) >>= _))] =>
-      iApply wsim_io; iIntros "%"
-  | [ |- environments.envs_entails _ (wsim _ _ _ _ _ _ _ _ _ _ _ (_, trigger GetTid >>= _) (_, trigger GetTid >>= _))] =>
-      iApply wsim_gettid; iIntros "%"
-  end.
-
-Ltac wstep :=
-  norm with do 1 _wstep; s; des_pairs; s.
-
-Ltac _wforce_l :=
-  match goal with
-  | [ |- environments.envs_entails _ (wsim _ _ _ _ _ _ _ _ _ _ _ (_, trigger (Choose ?T) >>= _) _) ] =>
-      iApply wsim_choose_src
-  | [ |- environments.envs_entails _ (wsim _ _ _ _ _ _ _ _ _ _ _ (_, trigger (Guarantee ?P) >>= _) _) ] =>
-      unfold_pre_post_term P; iApply wsim_guarantee_src
-      (* first [
-        tcsearch constr:(WP P)
-          ltac:(fun c =>
-          iApply (wsim_guarantee_src_WP _ _ _ _ _ _ _ _ _ _ _ _ _ _ _ (i:=c)); [try set_solver|try set_solver|simpl WP_space]);
-        match goal with
-        | [ |- environments.envs_entails _ (?P' ∗ _)] =>
-          unfold_pre_post_term P'
-        end
-      | unfold_pre_post_term P; iApply wsim_guarantee_src
-      ] *)
-  | [ |- environments.envs_entails _ (wsim _ _ _ _ _ _ _ _ _ _ _ (_, unwrapN _ >>= _) _) ] =>
-      iApply wsim_unwrapN_src
-  | [ |- environments.envs_entails _ (wsim _ _ _ _ _ _ _ _ _ _ _ (_, guarantee _ >>= _) _) ] =>
-      iApply wsim_guar_src
-  end.
-
-Ltac wforce_l_core :=
-  norm_l with do 1 _wforce_l.
-
-Tactic Notation "wforce_l" :=
-  wforce_l_core; [..|try iExists _].
-
-Tactic Notation "wforce_l" uconstr(p) :=
-  wforce_l_core; [..|iExists p].
-
-Ltac wforces_l :=
-  hrepeat do 1 wforce_l.
-
-Ltac _wforce_r :=
-  match goal with
-  | [ |- environments.envs_entails _ (wsim _ _ _ _ _ _ _ _ _ _ _ _ (_, trigger (Take _) >>= _)) ] =>
-      iApply wsim_take_tgt
-  | [ |- environments.envs_entails _ (wsim _ _ _ _ _ _ _ _ _ _ _ _ (_, trigger (Assume ?P) >>= _)) ] =>
-      (* first [
-        tcsearch constr:(WP P)
-          ltac:(fun c =>
-            unshelve iApply (wsim_assume_tgt_WP _ _ _ _ _ _ _ _ _ _ _ _ _ _ _ (i:=c)); s;
-            [first [apply nclose_subseteq|try set_solver]
-            |first [apply nclose_subseteq|try set_solver]
-            |simpl WP_space]
-          );
-        match goal with
-        | [ |- environments.envs_entails _ (?P' ∗ _)] =>
-          unfold_pre_post_term P'
-        end
-      | unfold_pre_post_term P; iApply wsim_assume_tgt ] *)
-    unfold_pre_post_term P; iApply wsim_assume_tgt
-  | [ |- environments.envs_entails _ (wsim _ _ _ _ _ _ _ _ _ _ _ _ (_, trigger (AssumeRes _) >>= _)) ] =>
-      iApply wsim_assume_res_tgt
-  | [ |- environments.envs_entails _ (wsim _ _ _ _ _ _ _ _ _ _ _ _ (_, assume _ >>= _)) ] =>
-      iApply wsim_asm_tgt
-  | [ |- environments.envs_entails _ (wsim _ _ _ _ _ _ _ _ _ _ _ _ (_, RealUpdate ?P ?Q >>= _)) ] =>
-      unfold_pre_post_term P; unfold_pre_post_term Q; iApply wsim_ru_tgt_simple
-  end
-.
-
-Ltac wforce_r_core :=
-  norm_r with do 1 _wforce_r; s.
-
-Tactic Notation "wforce_r" :=
-  wforce_r_core; try (iExists _).
-
-Tactic Notation "wforce_r" uconstr(p) :=
-  wforce_r_core; iExists p.
-
-Ltac wforces_r :=
-  hrepeat do 1 wforce_r.
-
-Ltac winline_l :=
-  norm_l with
-    do 1 iApply wsim_inline_src; [try prove_inline_cond|unfold_cris_defs].
-
-Ltac winline_r :=
-  norm_r with
-    do 1 iApply wsim_inline_tgt; [try prove_inline_cond|try prove_sb_cond|unfold_cris_defs].
-
-Ltac wcall hyps :=
-  (norm with do 1 iApply wsim_call); [try prove_sb_cond|
-  iSplitL hyps; [try done| iIntros "% % %"; iIntrosFresh "IST"];
-  move_aux].
-
-Ltac wspawn :=
-  (norm with do 1 iApply wsim_spawn); [try prove_sb_cond|].
-
-Ltac wyield hyps :=
-  (norm with do 1 iApply wsim_yield);
-  iSplitL hyps; [try done| iIntros "% %"; iIntrosFresh "IST"];
-  move_aux.
-
-Ltac wby_coind CIH :=
-  iApply wsim_progress; iApply wsim_base; iIntrosFresh "I";
-  iApply CIH.
-
-Ltac winit_simF :=
-  initialize_simF;
-  iApply wsim_isim;
-  try (
-      iDestruct "IST" as "[% [W [TID IST]]]"; des; subst;
-      iApply wsim_init_winv; iSplitL "W"; [et; fail|]; hss_copset;
-      hrepeat do 1 (unfold_mod; s)).
-
-  Ltac step_l := iwcase (do 1 istep_l) (do 1 wstep_l).
-  Ltac steps_l := iwcase (do 1 isteps_l) (do 1 wsteps_l).
-
-  Ltac step_r := iwcase (do 1 istep_r) (do 1 wstep_r).
-  Ltac steps_r := iwcase (do 1 isteps_r) (do 1 wsteps_r).
-
-  Ltac step := iwcase (do 1 istep) (do 1 wstep).
-
-  Tactic Notation "force_l" := iwcase (do 1 iforce_l) (do 1 wforce_l).
-  Tactic Notation "force_l" uconstr(p) := iwcase (do 1 iforce_l p) (do 1 wforce_l p).
-  Ltac forces_l := iwcase (do 1 iforces_l) (do 1 wforces_l).
-
-  Tactic Notation "force_r" := iwcase (do 1 iforce_r) (do 1 wforce_r).
-  Tactic Notation "force_r" uconstr(p) := iwcase (do 1 iforce_r p) (do 1 wforce_r p).
-  Ltac forces_r := iwcase (do 1 iforces_r) (do 1 wforces_r).
-
-  Ltac inline_l := iwcase (do 1 iinline_l) (do 1 winline_l).
-  Ltac inline_r := iwcase (do 1 iinline_r) (do 1 winline_r).
-  Ltac unfold_cris_defs :=
-    rewrite /SB.sandbox_body; s;
-    (hrepeat do 1 match goal with |- context[cfunU ?x] => rewrite {1}/x end);
-    rewrite /cfunU;
-    (hrepeat do 1 match goal with |- context[cfunN ?x] => rewrite {1}/x end);
-    rewrite /cfunN;
-    rewrite /SModTr.trans_fnsem.
-  (* TEMP *)
-
-  Lemma wsim_HoareFun_src fsp msk fbd arg fl_src fl_tgt Ist RR r g ps pt st_src st_tgt itr_tgt :
-    (∀ N tid x varg, TID tid -∗
-      YIELD tid -∗
-      precond fsp (N, tid) x varg arg -∗
-      wsim fl_src fl_tgt Ist (↑N, ↑N) r g Any.t Any.t
-        (λ src tgt, TID tid ∗ YIELD tid ∗ winv (↑N, ↑N) ∗
-          ∃ ret, postcond fsp (N, tid) x src.2 ret ∗ RR (src.1, ret) tgt) true pt
-        (st_src, SB.sandbox msk (fbd N tid varg))
-        (st_tgt, itr_tgt)) ⊢
-    wsim fl_src fl_tgt Ist (∅, ∅) r g Any.t Any.t RR ps pt
-      (st_src, SB.sandbox msk (SModTr.HoareFun (Some fsp) fbd arg))
-      (st_tgt, itr_tgt).
-  Proof.
-    iIntros "sim".
-    rewrite /SModTr.HoareFun.
-    norm_l. des_if; step_l; ss. destruct _q as [N tid].
-    steps_l. des_if; step_l; ss. rename _q into m.
-    steps_l. des_if; step_l; ss. rename _q into varg.
-    steps_l. des_if; step_l; ss.
-    iDestruct "ASM" as "[? [? W]]"; iApply wsim_fold; iFrame "W".
-    steps_l. des_if; step_l; ss. steps_l.
-    rewrite {2}(bind_ret_r_rev itr_tgt).
-    iPoseProof ("sim" with "[$] [$] [$]") as "sim".
-    iApply wsim_bind; iFrame "sim".
-    clear dependent st_src st_tgt.
-    iIntros (st_src r_s st_tgt r_t) "[? [? [W [%ret [Post RR]]]]]".
-    steps_l. des_ifs; steps_l; ss.
-    force_l ret. steps_l. des_ifs; steps_l; ss.
-    forces_l. iFrame. steps_l. des_ifs; steps_l; ss. force_l. iFrame "Post". step.
-  Qed.
-
-  Ltac iStartSim := init_simF; unfold_cris_defs; iApply wsim_HoareFun_src; eauto; ss.
 
   Lemma simF_alloc : ISim.sim_fun open MemA MemI IstFull (Some MemHdr.alloc).
   Proof using.
@@ -1101,14 +272,14 @@ Ltac winit_simF :=
     iPureIntro; esplits; eauto; cycle 1.
     { ii; ss. unfold update in *. rewrite /mem_wf in H6. des_ifs. exploit H6; eauto. nia. }
 
-    intros blk' ofs'; rewrite ?discrete_fun_lookup_op /= Z.add_0_l Z.sub_0_r repeat_length.
+    intros blk' ofs'; rewrite ?discrete_fun_lookup_op /= Z.add_0_l Z.sub_0_r length_replicate.
     destruct (mem_tgt.(Mem.cnts) blk ofs') eqn:E.
     { exfalso. exploit H6; et. nia. }
     ss. hexploit (H5 blk ofs'); et.
     rewrite E. intro U. des; ss.
 
     case_bool_decide as Hblkofs; [destruct Hblkofs as [Hblk Hofs]|].
-    { rewrite repeat_nth_some; [subst|lia]; rewrite U left_id; right; esplits; eauto.
+    { rewrite lookup_replicate_2; [subst|lia]; rewrite U left_id; right; esplits; eauto.
       rewrite /update; destruct (dec _ _); ss; case_bool_decide; ss.
     }
     rewrite right_id /update; destruct (_ blk' ofs') eqn : ?; hexploit (H5 blk' ofs');
@@ -1257,7 +428,7 @@ Ltac winit_simF :=
         uo; des_ifs; bsimpl; des; des_sumbool; subst; ss; rewrite ?Heq0 ?Heq1 ?Heq2; des_ifs; et.
       }
       { ii. revert H1. rewrite /Mem.load_mem; uo; s. des_ifs.
-        i. inv H1. eapply nth_error_Some. destruct (nth_error genv b); ss.
+        i. inv H1. eapply lookup_lt_Some; eauto.
       }
     }
     { intros fn; eapply ISim.sim_fun_strong; rewrite !dom_fmap /= /MemA.fnsems ?dom_insert_L;
