imp_system/mem/MemTactics.v
@@ -4,26 +4,25 @@ Require Export ImpPrelude MemHeader MemA.
 Section mem.
   Context `{!crisG Γ Σ α β τ _S _I, !concG, !memG}.
 
-  Local Definition state : Type := alist key Any.t.
+  Local Definition state : Type := gmap key (option Any.t).
   Local Definition post (R_s R_t : Type) : Type := state * R_s → state * R_t → iProp Σ.
   Local Definition rel : Type := ∀ R_s R_t : Type,
     post R_s R_t → bool → bool → state * itree crisE R_s → state * itree crisE R_t → iProp Σ.
 
-  Context (fl_s fl_t : alist (option string) (Any.t → itree crisE Any.t)).
-  Context (Ist : alist key Any.t → alist key Any.t → iProp Σ).
+  Context (fl_s fl_t : gmap (option string) (option (Any.t → itree crisE Any.t))).
+  Context (Ist : gmap key (option Any.t) → gmap key (option Any.t) → iProp Σ).
   Context (R_s R_t : Type).
   Context (RR : post R_s R_t).
   Context (ps pt : bool).
   Context (st_src st_tgt : state).
 
-  Context (sp: sp_type).
+  Context (sp : specmap).
 
-  Lemma wsim_mem_alloc (sz : Z) k_s k_t E1 E2 r g img_t msk_t scp_t msk_m :
-    alist_find (Some MemHdr.alloc) fl_t =
-      Some (SB.sandbox_body
-        (SModTr.trans_ktree sp
-          (true, msk_m, MemA.scopes, (Some (to_fspec MemSpec.alloc), fbody_trivial)))) →
-    (msk_t MemHdr.alloc : bool) →
+  Lemma wsim_mem_alloc (sz : Z) k_s k_t E1 E2 r g :
+    fl_t !! (Some MemHdr.alloc) =
+      Some (Some (SB.sandbox_body
+        (msk_scp MemA.scopes msk_true,
+         SModTr.trans_fnsem sp (Some MemSpec.alloc, fbody_trivial)))) →
     (0 <= 8 * sz < modulus_64)%Z →
     (∀ blk,
       ([∗ list] i ↦ v ∈ repeat Vundef (Z.to_nat sz), (blk, Z.of_nat i)%Z ↦ v) -∗
@@ -32,22 +31,23 @@ Section mem.
       (st_tgt, k_t (Vptr (blk, 0%Z))↑)) ⊢
     wsim fl_s fl_t Ist (E1, E2) r g R_s R_t RR ps pt
       (st_src, k_s)
-      (st_tgt, x <- (SB.sandbox img_t msk_t scp_t (trigger (Call MemHdr.alloc [Vint sz]↑)));; k_t x).
+      (st_tgt, x <- (trigger (Call MemHdr.alloc [Vint sz]↑));; k_t x).
   Proof.
-    intros Hin Hmsk Hsz.
+  Admitted.
+    (* intros Hin Hsz.
     iIntros "K".
     inline_r. steps_r. force_r (Z.to_nat sz). forces_r. iSplit; eauto.
     { rewrite Z2Nat.id //; try lia. iSplit; eauto. iSplit; eauto. iPureIntro; lia. }
     steps_r. iDestruct "GRT" as "[[% [-> ↦]] ->]". iApply "K".
     iApply (big_sepL_impl with "↦").
     iIntros "!> % % %"; rewrite Z.add_0_l; iIntros "$".
-  Qed.
+  Qed. *)
 
-  Lemma wsim_mem_store b ofs v v' k_s k_t E1 E2 r g img_t msk_t scp_t msk_m :
+  (* Lemma wsim_mem_store b ofs v v' k_s k_t E1 E2 r g img_t msk_t scp_t msk_m :
     alist_find (Some MemHdr.store) fl_t =
       Some (SB.sandbox_body
-        (SModTr.trans_ktree sp
-          (true, msk_m, MemA.scopes, (Some (to_fspec MemSpec.store), fbody_trivial)))) →
+        (SModTr.trans_fnsem sp
+          (true, msk_m, MemA.scopes, (Some (MemSpec.store), fbody_trivial)))) →
     (msk_t MemHdr.store : bool) →
     (b, ofs) ↦ v' -∗
     ((b, ofs) ↦ v -∗
@@ -69,8 +69,8 @@ Section mem.
   Lemma wsim_mem_load b ofs q v k_s k_t E1 E2 r g img_t msk_t scp_t msk_m :
     alist_find (Some MemHdr.load) fl_t =
       Some (SB.sandbox_body
-        (SModTr.trans_ktree sp
-          (true, msk_m, MemA.scopes, (Some (to_fspec MemSpec.load), fbody_trivial)))) →
+        (SModTr.trans_fnsem sp
+          (true, msk_m, MemA.scopes, (Some (MemSpec.load), fbody_trivial)))) →
     (msk_t MemHdr.load : bool) →
     (b, ofs) ↦{q} v -∗
     ((b, ofs) ↦{q} v -∗
@@ -92,8 +92,8 @@ Section mem.
   Lemma wsim_mem_cas b ofs v v_old v_new succ E k_s k_t E1 E2 r g img_t msk_t scp_t msk_m :
     alist_find (Some MemHdr.cas) fl_t =
       Some (SB.sandbox_body
-        (SModTr.trans_ktree sp
-          (true, msk_m, MemA.scopes, (Some (to_fspec MemSpec.cas), fbody_trivial)))) →
+        (SModTr.trans_fnsem sp
+          (true, msk_m, MemA.scopes, (Some (MemSpec.cas), fbody_trivial)))) →
     (msk_t MemHdr.cas : bool) →
     MemSpec.compare_val v v_old = Vint succ →
     (b, ofs) ↦ v -∗
@@ -122,8 +122,8 @@ Section mem.
   Lemma wsim_mem_cmp v1 v2 succ E k_s k_t E1 E2 r g img_t msk_t scp_t msk_m :
     alist_find (Some MemHdr.cmp) fl_t =
       Some (SB.sandbox_body
-        (SModTr.trans_ktree sp
-          (true, msk_m, MemA.scopes, (Some (to_fspec MemSpec.cmp), fbody_trivial)))) →
+        (SModTr.trans_fnsem sp
+          (true, msk_m, MemA.scopes, (Some (MemSpec.cmp), fbody_trivial)))) →
     (msk_t MemHdr.cmp : bool) →
     MemSpec.compare_val v1 v2 = Vint succ →
     E -∗
@@ -145,5 +145,5 @@ Section mem.
     inline_r. steps_r. force_r (v1, v2, succ, E). forces_r.
     iFrame "E HE"; iSplit; eauto.
     steps_r. iDestruct "GRT" as "[[-> E] ->]". iApply ("K" with "E"); iFrame.
-  Qed.
+  Qed. *)
 End mem.
