theories/simulations/ctxrefine/CtxRefineFacts.v
@@ -1,362 +1,185 @@
-Require Import Common.
 From iris.proofmode Require Import proofmode.
+Require Import Common.
 Require Import Mod.
 Require Import MSimCommon ISim ISimFacts.
 Require Import CtxRefine MainAdequacy.
 Require Import Tactics TacticsInit.
 
-(* Set Implicit Arguments. *)
-
-(*******
-  Commutativity Proof
- *******)
-
-(* Definition perm_Ist `{Σ: GRA} : alist key Any.t -> alist key Any.t -> iProp Σ :=
-  λ l0 l1, ⌜l0 ≡ₚ l1⌝%I.  
-
-Lemma alist_upd_perm {K V} l0 l1 `{Dec K} (k : K) (v : V)
-    (ND : List.NoDup (List.map fst l0))
-    (PERM : l0 ≡ₚ l1) :
-  alist_upd k v l0 ≡ₚ alist_upd k v l1.
-Proof.
-  destruct (classic (In k (List.map fst l0))); cycle 1.
-  {
-    rewrite! alist_upd_not_in; eauto. ii.
-    eapply H0. eapply Permutation_in; cycle 1; eauto.
-    eapply Permutation_map. symmetry. eauto.
-  }
-  assert (List.NoDup (List.map fst l1)).
-  { 
-    eapply Permutation_NoDup; cycle 1; eauto. 
-    eapply Permutation_map. eauto.
-  }
-  eapply alist_find_fst_in in H0. des.
-  eapply alist_find_some in H0.
-  assert (In (k, v0) l1).
-  { eapply Permutation_in; eauto. }
-  eapply in_split in H0, H2. des. subst.
-  replace (l4 ++ (k, v0) :: l5) with ((l4 ++ [(k, v0)] ++ l5)); eauto.
-  replace (l2 ++ (k, v0) :: l3) with ((l2 ++ [(k, v0)] ++ l3)); eauto.
-  rewrite! alist_upd_with_nodup; eauto.
-  eapply Permutation_app_middle, Permutation_app_inv. eauto.
-  Unshelve. eauto.
-Qed.
-
-Lemma alist_permutation_find K `{Dec K} V (l0 l1 : alist K V)
-      (ND : List.NoDup (List.map fst l0))
-      (PERM : Permutation l0 l1)
-      k
-  :
-    alist_find k l0 = alist_find k l1.
-Proof.
-  revert ND k. induction PERM; ss.
-  { i. inv ND. destruct x. rewrite eq_rel_dec_correct. des_ifs. et. }
-  { i. inv ND. inv H3. destruct x, y. rewrite eq_rel_dec_correct. des_ifs.
-    rewrite eq_rel_dec_correct in Heq0. des_ifs. f_equal. exfalso. eapply H2. ss. auto. }
-  { i. rewrite IHPERM1; auto. rewrite IHPERM2; auto.
-    eapply Permutation_NoDup; [|apply ND].
-    eapply Permutation_map. auto.
-  }
-Qed.
-
-Lemma alist_find_comm {K V} `{Dec K}
-      (l0 l1 : list (K*V)) fn f
-      (NODUP : List.NoDup (List.map fst (l0 ++ l1)))
-      (FIND : alist_find fn (l0 ++ l1) = Some f)
-    :
-      alist_find fn (l1 ++ l0) = Some f.
-Proof.
-  move: FIND; rewrite ?alist_find_app_o; intros FIND. des_ifs.
-  eapply alist_find_fst_some in Heq, Heq0.
-  rewrite map_app in NODUP.
-  exfalso.
-  eapply NoDup_app_disjoint in NODUP; eauto.
-Qed. *)
-
+(** Properties of contextual refinement *)
 Section CtxRefineFacts.
   Context `{_crisG: !crisG Γ Σ α β τ _S _I}.
 
-  (* Lemma mod_add_scopes md0 md1:
-    Mod.scopes (md0 ★ md1) = Mod.scopes md0 ++ Mod.scopes md1.
-  Proof using. ss. Qed. *)
+  Global Program Instance refines_mod_PreOrder : PreOrder (@refines_lmod).
+  Next Obligation. ii. ss. Qed.
+  Next Obligation. ii. eapply H. eapply H0. ss. Qed.
 
-  (* Lemma mod_add_comm contextual (ms0 ms1 : Mod.t) :
-    ISim.t contextual (ms0 ★ ms1) (ms1 ★ ms0) emp%I (IstSB (Mod.scopes (ms0 ★ ms1)) IstEq).
+  Global Program Instance refines_PreOrder : PreOrder refines.
+  Next Obligation.
+    ii. esplits; eauto. ii. esplits; eauto. refl.
+  Qed.
+  Next Obligation.
+    ii.
+    edestruct H; eauto; edestruct H0; eauto. des.
+    esplits; eauto. ii.
+    specialize (H2 rs WFR SRC). des.
+    specialize (H4 rt H2 H5). des. 
+    exists rt0. esplits; eauto.
+    etrans; eauto.
+  Qed.
+
+  (*** vertical composition ***)
+  Global Program Instance ctx_refines_PreOrder : PreOrder ctx_refines.
+  Next Obligation. r. r. i. refl. Qed.
+  Next Obligation.
+    r. r. i. etrans.
+    - apply H.
+    - apply H0.
+  Qed.
+
+  Global Program Instance ctx_refines_Proper : Proper ((≡) ==> (≡) ==> iff) ctx_refines.
+  Next Obligation.
+    intros ms1 ms2 mseq mt1 mt2 mteq; split; intros CTXR.
+    { destruct ms1, ms2, mt1, mt2; inv mseq; inv mteq; ii; ss; split; auto; clarify.
+      { apply CTXR; s; eauto. }
+      { ii. destruct (CTXR _ WFM). hexploit (H1 rs); eauto; ss.
+        { rewrite H0; done. }
+        { intros [rt Hrt]; rewrite H2 in Hrt; des; exists rt; esplits; eauto. }
+      }
+    }
+    { destruct ms1, ms2, mt1, mt2; inv mseq; inv mteq; ii; ss; split; auto; clarify.
+      { apply CTXR; s; eauto. }
+      { ii. destruct (CTXR _ WFM). hexploit (H1 rs); eauto; ss.
+        { rewrite -H0; done. }
+        { intros [rt Hrt]; rewrite -H2 in Hrt; des; exists rt; esplits; eauto. }
+      }
+    }
+  Qed.
+
+  Global Program Instance ctx_refines_Proper2 mc : Proper ((≡) ==> iff) (ctx_refines mc).
+  Next Obligation.
+    i. eapply ctx_refines_Proper. et.
+  Qed.
+
+  Lemma ctxr_refines mcs mct (REF : ctx_refines mcs mct) :
+    refines mcs mct.
   Proof using.
-    econs; ss; intros Hwf.
-    { apply Permutation_submseteq, Permutation_app_comm. }
-    { iIntros "_"; iSplit; cycle 1.
-      { iPureIntro. eapply fin_maps.union_with_comm; ss. }
-      { admit. }
-    }
-  { rewrite ?map_app; i. apply sub_perm_comm. }
-  { ii. ss. rewrite !map_app !alist_find_app_o in H0 |- *.
-    des_ifs. esplits; et.
-    iPureIntro. i. esplits; et.
-    - rewrite /state_scopes map_app.
-      eapply incl_app; [apply incl_appl|apply incl_appr];
-        eapply Mod.well_scoped_init.
-    - rewrite /state_scopes map_app.
-      eapply incl_app; [apply incl_appr|apply incl_appl];
-        eapply Mod.well_scoped_init.
-    - eapply Permutation_app_comm.
-  }
+    i. specialize (REF Mod.empty_mc).
+    destruct mcs, mct. ss.
+    rewrite -!mod_add_empty_r in REF.
+    ii; split; ii; des; ss; red in REF; hexploit REF; eauto; i; des; ss.
+    hexploit (H0 rs); ss.
+    { rewrite SRC. iIntros ">[? ?]"; iFrame; et. }
+    i; des; esplits; eauto.
+    rewrite H2. iIntros ">[? [? ?]]". iFrame. et.
+  Qed.
 
-  destruct fn; cycle 1.
-  {
-    ii. ss. dup FIND.
-    eapply alist_find_comm in FIND0; et. rewrite FIND0. esplits; et.
-    ii. iIntros "% I". des; subst.
-    iApply isim_mono; cycle 1.
-    - iApply isim_refl.
-      + ii. iIntros "%". iPureIntro. des. eapply alist_permutation_find; et.
-      + ii. iIntros "%". iPureIntro. des. esplits; et.
-        * rewrite state_scopes_update. et.
-        * rewrite state_scopes_update. et.
-        * eapply alist_upd_perm; et.
-      + iPureIntro. esplits; et.
-        * rewrite /state_scopes map_app.
-          eapply incl_app; [apply incl_appl|apply incl_appr];
-            eapply Mod.well_scoped_init.
-        * rewrite /state_scopes map_app.
-          eapply incl_app; [apply incl_appr|apply incl_appl];
-            eapply Mod.well_scoped_init.
-        * eapply Permutation_app_comm.
-    - i. iIntros "%". iPureIntro. des; et.
-  }
+  (*** weakening for initial condition ***)
+  Lemma ctxr_cond_strengthen (m : Mod.t) (P Q : iProp Σ) (IMPL : P ⊢ Q) :
+    ctx_refines (m, P) (m, Q).
+  Proof using.
+    ii. ss; split; first done. ii; ss; exists rs. esplits; eauto.
+    + rewrite SRC IMPL. et.
+    + refl.
+  Qed.
 
-  ii. eapply alist_find_comm in FIND; et. rewrite FIND. esplits; et.
+  (*** frame rule for initial condition ***)
+  Lemma ctxr_cond_frameR (ms mt : Mod.t) Ps Pt Q (REF : ctx_refines (ms, Ps) (mt, Pt)) :
+    ctx_refines (ms, Ps ∗ Q)%I (mt, Pt ∗ Q)%I.
+  Proof using.
+    ii. specialize (REF (ctx.1, Q ∗ ctx.2)%I).
+    destruct ctx. ss.
+    split.
+    { red in REF. hexploit REF; ss; i; des; eauto. }
+    ii. ss. des. red in REF. hexploit REF; ss; i; des; eauto.
+    hexploit (H0 rs); ss.
+    { rewrite SRC. iIntros ">[? [[? ?] ?]]". iFrame. et. }
+    i; des; esplits; eauto.
+    rewrite H2. iIntros ">[? [? [? ?]]]". iFrame. et.
+  Qed.
 
-  (* simulation *)
-  ii. iIntros "S I". iStopProof.
-  destruct fs as [[[img msk] scp] bd]. unfold SB.sandbox_body. s.
-  generalize (bd arg) as it. clear FIND bd arg.
-  combine_quant st_tgt.
-  combine_quant st_src.
-  eapply isim_coind. intros g0 _ CIH [st_src [st_tgt it]].
-  destruct_quant CIH. iIntros "(%IST & I)". des.
-  assert (CASE := case_itrH it); des; subst.
-  - step. eauto.
-  - steps_l. steps_r. by_coind CIH; et.
-  - destruct img.
-    + steps_l. force_r. iFrame. steps_r. by_coind CIH; et.
-    + rewrite SBRed.bind SBRed.Assume. s. steps_l. ss.
-  - steps_l. force_r. iFrame. steps_l; steps_r. by_coind CIH; eauto.
-  - steps_r. force_l. iFrame. steps_l. by_coind CIH; et.
-  - destruct c.
-    + norm_l. norm_r. rewrite! SBRed.call. des_ifs; ss.
-      * iApply isim_call. iSplit; eauto. iIntros (???) "IST0".
-        steps_l. steps_r. by_coind CIH; et.
-      * steps_l. ss.
-    + norm_l. norm_r. rewrite! SBRed.spawn. des_ifs; ss.
-      * iApply isim_spawn. iIntros "%".
-        steps_l. steps_r. by_coind CIH; et.
-      * steps_l. ss.
-    + yield ""; eauto. by_coind CIH; et.
-    + step; eauto. by_coind CIH; et.
-  - iApply isim_nodup_src; iIntros (?).
-    depdes s0.
-    + rewrite !SBRed.bind !SBRed.put. des_ifs; cycle 1.
-      { steps_l. ss. }
-      iApply isim_sput_src. iApply isim_sput_tgt.
-      by_coind CIH; et.
-      iFrame. unfold perm_Ist. iPureIntro.
-      rewrite !state_scopes_update. esplits; eauto. 
-      eapply alist_upd_perm; eauto.
-    + rewrite !SBRed.bind !SBRed.get. des_ifs; cycle 1.
-      { steps_l. ss. }
-      iApply isim_sget_src. iApply isim_sget_tgt.
-      apply existsb_exists in Heq. des. apply String.eqb_eq in Heq0. subst.
-      iAssert (⌜alist_find k st_src = alist_find k st_tgt⌝)%I as "%".
-      { iPureIntro. eapply alist_permutation_find; eauto. }
-      rewrite H0. by_coind CIH; et.
-  - destruct e.
-    + steps_r. force_l. instantiate (1:= _q). steps_l. by_coind CIH; et.
-    + rewrite SBRed.bind SBRed.take. des_ifs.
-      * steps_l. force_r. instantiate (1:= _q). steps_r. by_coind CIH; et.
-      * steps_l. ss.
-    + step. by_coind CIH; et.
-Qed. *)
+  Lemma ctxr_cond_frameL (ms mt : Mod.t) Ps Pt Q (REF : ctx_refines (ms, Ps) (mt, Pt)) :
+    ctx_refines (ms, Q ∗ Ps)%I (mt, Q ∗ Pt)%I.
+  Proof using.
+    etrans; [|etrans]; cycle 1.
+    { apply ctxr_cond_frameR with (Q:=Q) in REF. apply REF. }
+    { eapply ctxr_cond_strengthen. i. iIntros "(H1 & H2)". iFrame. }
+    { eapply ctxr_cond_strengthen. i. iIntros "(H1 & H2)". iFrame. }
+  Qed.
 
-(*******
-  Properties of Contextual Refinements
- *******)
+  (*** commutativity ***)
+  Theorem ctxr_comm (ma mb : Mod.t) P:
+    ctx_refines (Mod.add ma mb, P) (Mod.add mb ma, P).
+  Proof using. rewrite Mod.add_comm //. Qed.
 
-Global Program Instance refines_mod_PreOrder : PreOrder (@refines_lmod).
-Next Obligation. ii. ss. Qed.
-Next Obligation. ii. eapply H. eapply H0. ss. Qed.
+  (*** frame rules ***)
+  Lemma ctxr_frameR ms Ps mt Pt mc (REFA : ctx_refines (ms, Ps) (mt, Pt)) :
+    ctx_refines (ms ★ mc, Ps) (mt ★ mc, Pt).
+  Proof using.
+    intro. specialize (REFA (Mod.add mc ctx.1, ctx.2)). ss.
+    move: REFA; rewrite !mod_add_assoc; eauto.
+  Qed.
 
-Global Program Instance refines_PreOrder : PreOrder refines.
-Next Obligation.
-  ii. esplits; eauto. ii. esplits; eauto. refl.
-Qed.
-Next Obligation.
-  ii.
-  edestruct H; eauto; edestruct H0; eauto. des.
-  esplits; eauto. ii.
-  specialize (H2 rs WFR SRC). des.
-  specialize (H4 rt H2 H5). des. 
-  exists rt0. esplits; eauto.
-  etrans; eauto.
-Qed.
+  Lemma ctxr_frameL ms Ps mt Pt mc (REFA : ctx_refines (ms, Ps) (mt, Pt)) :
+    ctx_refines (mc ★ ms, Ps) (mc ★ mt, Pt).
+  Proof using.
+    etrans. { eapply ctxr_comm. }
+    etrans. { eapply ctxr_frameR. apply REFA. }
+    apply ctxr_comm.
+  Qed.
 
-(*** vertical composition ***)
-Global Program Instance ctx_refines_PreOrder : PreOrder ctx_refines.
-Next Obligation. r. r. i. refl. Qed.
-Next Obligation.
-  r. r. i. etrans.
-  - apply H.
-  - apply H0.
-Qed.
+  (*** horizontal composition ***)
+  Lemma ctxr_compose_hor msa Psa mta Pta msb Psb mtb Ptb
+      (REFA : ctx_refines (msa, Psa) (mta, Pta))
+      (REFB : ctx_refines (msb, Psb) (mtb, Ptb)) :
+    ctx_refines (msa ★ msb, Psa ∗ Psb)%I
+                (mta ★ mtb, Pta ∗ Ptb)%I.
+  Proof using.
+    etrans.
+    - eapply ctxr_frameR, ctxr_cond_frameR. apply REFA.
+    - eapply ctxr_frameL, ctxr_cond_frameL. apply REFB. 
+  Qed.
 
-Global Program Instance ctx_refines_Proper : Proper ((≡) ==> (≡) ==> iff) ctx_refines.
-Next Obligation.
-  intros ms1 ms2 mseq mt1 mt2 mteq; split; intros CTXR.
-  { destruct ms1, ms2, mt1, mt2; inv mseq; inv mteq; ii; ss; split; auto; clarify.
-    { apply CTXR; s; eauto. }
-    { ii. destruct (CTXR _ WFM). hexploit (H1 rs); eauto; ss.
-      { rewrite H0; done. }
-      { intros [rt Hrt]; rewrite H2 in Hrt; des; exists rt; esplits; eauto. }
-    }
-  }
-  { destruct ms1, ms2, mt1, mt2; inv mseq; inv mteq; ii; ss; split; auto; clarify.
-    { apply CTXR; s; eauto. }
-    { ii. destruct (CTXR _ WFM). hexploit (H1 rs); eauto; ss.
-      { rewrite -H0; done. }
-      { intros [rt Hrt]; rewrite -H2 in Hrt; des; exists rt; esplits; eauto. }
-    }
-  }
-Qed.
+  (*** mixed composition ***)
+  Lemma ctxr_compose_mix msa Psa mta Pta msb Psb mtb Ptb mc
+      (REFA : ctx_refines (msa ★ mc, Psa) (mta ★ mc, Pta))
+      (REFB : ctx_refines (msb ★ mc, Psb) (mtb ★ mc, Ptb)) :
+    ctx_refines (msa ★ msb ★ mc, Psa ∗ Psb)%I
+                (mta ★ mtb ★ mc, Pta ∗ Ptb)%I.
+  Proof using.
+    etrans.
+    { eapply ctxr_frameL, ctxr_cond_frameL. apply REFB. }
+    etrans.
+    { eapply ctxr_frameL, ctxr_comm. }
+    etrans.
+    { rewrite <-mod_add_assoc.
+      eapply ctxr_frameR, ctxr_cond_frameR. apply REFA. }
+    rewrite mod_add_assoc.
+    apply ctxr_frameL, ctxr_comm.
+  Qed.
 
-Global Program Instance ctx_refines_Proper2 mc : Proper ((≡) ==> iff) (ctx_refines mc).
-Next Obligation.
-  i. eapply ctx_refines_Proper. et.
-Qed.
+  (*** Corollaries for tactics ***)
 
-Lemma ctxr_refines mcs mct (REF : ctx_refines mcs mct) :
-  refines mcs mct.
-Proof using.
-  i. specialize (REF Mod.empty_mc).
-  destruct mcs, mct. ss.
-  rewrite -!mod_add_empty_r in REF.
-  ii; split; ii; des; ss; red in REF; hexploit REF; eauto; i; des; ss.
-  hexploit (H0 rs); ss.
-  { rewrite SRC. iIntros ">[? ?]"; iFrame; et. }
-  i; des; esplits; eauto.
-  rewrite H2. iIntros ">[? [? ?]]". iFrame. et.
-Qed.
+  Corollary ctxr_compose_hor_simplR msa mta msb mtb P Pa
+      (REFA : ctx_refines (msa, Pa) (mta, P))
+      (REFB : ctx_refines (msb, emp%I) (mtb, emp%I)) :
+    ctx_refines (msa ★ msb, Pa)%I
+                (mta ★ mtb, P)%I.
+  Proof using.
+    rewrite (mod_addc_empty_r _ P) (mod_addc_empty_r _ Pa).
+    eapply ctxr_compose_hor; et.
+  Qed.
 
-(*** weakening for initial condition ***)
-Lemma ctxr_cond_strengthen (m : Mod.t) (P Q : iProp Σ) (IMPL : P ⊢ Q) :
-  ctx_refines (m, P) (m, Q).
-Proof using.
-  ii. ss; split; first done. ii; ss; exists rs. esplits; eauto.
-  + rewrite SRC IMPL. et.
-  + refl.
-Qed.
-
-(*** frame rule for initial condition ***)
-Lemma ctxr_cond_frameR (ms mt : Mod.t) Ps Pt Q (REF : ctx_refines (ms, Ps) (mt, Pt)) :
-  ctx_refines (ms, Ps ∗ Q)%I (mt, Pt ∗ Q)%I.
-Proof using.
-  ii. specialize (REF (ctx.1, Q ∗ ctx.2)%I).
-  destruct ctx. ss.
-  split.
-  { red in REF. hexploit REF; ss; i; des; eauto. }
-  ii. ss. des. red in REF. hexploit REF; ss; i; des; eauto.
-  hexploit (H0 rs); ss.
-  { rewrite SRC. iIntros ">[? [[? ?] ?]]". iFrame. et. }
-  i; des; esplits; eauto.
-  rewrite H2. iIntros ">[? [? [? ?]]]". iFrame. et.
-Qed.
-
-Lemma ctxr_cond_frameL (ms mt : Mod.t) Ps Pt Q (REF : ctx_refines (ms, Ps) (mt, Pt)) :
-  ctx_refines (ms, Q ∗ Ps)%I (mt, Q ∗ Pt)%I.
-Proof using.
-  etrans; [|etrans]; cycle 1.
-  { apply ctxr_cond_frameR with (Q:=Q) in REF. apply REF. }
-  { eapply ctxr_cond_strengthen. i. iIntros "(H1 & H2)". iFrame. }
-  { eapply ctxr_cond_strengthen. i. iIntros "(H1 & H2)". iFrame. }
-Qed.
-
-(*** commutativity ***)
-Theorem ctxr_comm (ma mb : Mod.t) P:
-  ctx_refines (Mod.add ma mb, P) (Mod.add mb ma, P).
-Proof using. rewrite Mod.add_comm //. Qed.
-
-(*** frame rules ***)
-Lemma ctxr_frameR ms Ps mt Pt mc (REFA : ctx_refines (ms, Ps) (mt, Pt)) :
-  ctx_refines (ms ★ mc, Ps) (mt ★ mc, Pt).
-Proof using.
-  intro. specialize (REFA (Mod.add mc ctx.1, ctx.2)). ss.
-  move: REFA; rewrite !mod_add_assoc; eauto.
-Qed.
-
-Lemma ctxr_frameL ms Ps mt Pt mc (REFA : ctx_refines (ms, Ps) (mt, Pt)) :
-  ctx_refines (mc ★ ms, Ps) (mc ★ mt, Pt).
-Proof using.
-  etrans. { eapply ctxr_comm. }
-  etrans. { eapply ctxr_frameR. apply REFA. }
-  apply ctxr_comm.
-Qed.
-
-(*** horizontal composition ***)
-Lemma ctxr_compose_hor msa Psa mta Pta msb Psb mtb Ptb
-    (REFA : ctx_refines (msa, Psa) (mta, Pta))
-    (REFB : ctx_refines (msb, Psb) (mtb, Ptb)) :
-  ctx_refines (msa ★ msb, Psa ∗ Psb)%I
-              (mta ★ mtb, Pta ∗ Ptb)%I.
-Proof using.
-  etrans.
-  - eapply ctxr_frameR, ctxr_cond_frameR. apply REFA.
-  - eapply ctxr_frameL, ctxr_cond_frameL. apply REFB. 
-Qed.
-
-(*** mixed composition ***)
-Lemma ctxr_compose_mix msa Psa mta Pta msb Psb mtb Ptb mc
-    (REFA : ctx_refines (msa ★ mc, Psa) (mta ★ mc, Pta))
-    (REFB : ctx_refines (msb ★ mc, Psb) (mtb ★ mc, Ptb)) :
-  ctx_refines (msa ★ msb ★ mc, Psa ∗ Psb)%I
-              (mta ★ mtb ★ mc, Pta ∗ Ptb)%I.
-Proof using.
-  etrans.
-  { eapply ctxr_frameL, ctxr_cond_frameL. apply REFB. }
-  etrans.
-  { eapply ctxr_frameL, ctxr_comm. }
-  etrans.
-  { rewrite <-mod_add_assoc.
-    eapply ctxr_frameR, ctxr_cond_frameR. apply REFA. }
-  rewrite mod_add_assoc.
-  apply ctxr_frameL, ctxr_comm.
-Qed.
-
-(*** Corollaries for tactics ***)
-
-Corollary ctxr_compose_hor_simplR msa mta msb mtb P Pa
-    (REFA : ctx_refines (msa, Pa) (mta, P))
-    (REFB : ctx_refines (msb, emp%I) (mtb, emp%I)) :
-  ctx_refines (msa ★ msb, Pa)%I
-              (mta ★ mtb, P)%I.
-Proof using.
-  rewrite (mod_addc_empty_r _ P) (mod_addc_empty_r _ Pa).
-  eapply ctxr_compose_hor; et.
-Qed.
-
-Corollary ctxr_cond_frameR_simpl (ms mt : Mod.t) P Q
-  (REF : ctx_refines (ms, P) (mt, emp%I))
-  :
-  ctx_refines (ms, P ∗ Q)%I (mt, Q)%I.
-Proof using.
-  rewrite (mod_addc_empty_l _ Q).
-  eapply ctxr_cond_frameR. et.
-Qed.
-
+  Corollary ctxr_cond_frameR_simpl (ms mt : Mod.t) P Q
+    (REF : ctx_refines (ms, P) (mt, emp%I))
+    :
+    ctx_refines (ms, P ∗ Q)%I (mt, Q)%I.
+  Proof using.
+    rewrite (mod_addc_empty_l _ Q).
+    eapply ctxr_cond_frameR. et.
+  Qed.
 End CtxRefineFacts.
 
-(*******
- tactics for composing ctx_refines
- *******)
-
+(** tactics for composing ctx_refines *)
 Ltac ctxr_norm :=
   try rewrite <-!mod_add_assoc;
   try rewrite ->!mod_add_assoc;
