theories/simulations/msim/TacticsInit.v
@@ -1,22 +1,22 @@
-Require Import Common.
+Require Import Common ConcRA.
 From iris.proofmode Require Export proofmode.
-Require Import Mod ISim ISimFacts SModTr.
-Require Import TacticsCommon ITactics.
+Require Import TacticsCommon ITactics WTactics Tactics.
+Require Import Mod ISim WSim SModTr.
 
 (***
  Module-level tactics
  ***)
 
-Ltac hide_flist :=
+(* Ltac hide_flist :=
   let FLS := fresh "FLS" in let FLT := fresh "FLT" in
   match goal with [|- context[(isim_fsem ?fls ?flt)]] =>
     set (FLS := fls); set (FLT := flt)
-  end.
+  end. *)
 
-Ltac kill_trivial :=
-  match goal with |-?T => match type of T with Prop => econs; fail end end.
+(* Ltac kill_trivial :=
+  match goal with |-?T => match type of T with Prop => econs; fail end end. *)
 
-Ltac clear_trivials :=
+(* Ltac clear_trivials :=
   (hrepeat do 1
    lazymatch goal with H: ?T |-_ =>
      revert H; 
@@ -25,32 +25,32 @@ Ltac clear_trivials :=
        assert (TMP: T) by (econs; fail); clear TMP; intros []; []
      end
    end);
-  i.
+  i. *)
 
-Ltac pre_simF :=
+(* Ltac pre_simF :=
   clear_trivials;
   unfold ISim.sim_fun; i;
   match goal with [H: _|-_] => revert H end;
-  hide_flist.
+  hide_flist. *)
 
-Ltac post_simF :=
+(* Ltac post_simF :=
   eexists; split; [eauto|];
   ii; subst; iIntros "IST";
   unfold_cris_defs;
-  move_aux.
+  move_aux. *)
 
-Ltac initialize_simF :=
+(* Ltac initialize_simF :=
   pre_simF;
   alist_find_simpl;
   let H := fresh "H" in intro H; eapply some_injective in H; subst;
   alist_find_simpl;
-  post_simF.
+  post_simF. *)
 
-Ltac unfold_mod_fn :=
+(* Ltac unfold_mod_fn :=
   s; match goal with
      | |-context[_ \/ _] => idtac
      | _ => unfold_mod; ss; unfold_mod_fn
-     end.
+     end. *)
 
 (* Ltac prove_ist :=
   i; first [iIntros "->" | iIntros "[% ->]"];
@@ -58,7 +58,7 @@ Ltac unfold_mod_fn :=
   try rewrite state_scopes_update;
   et. *)
 
-Ltac init_sim :=
+(* Ltac init_sim :=
   clear_trivials;
   (first
   [ eapply ISim_reflR;
@@ -74,6 +74,44 @@ Ltac init_sim :=
     | r; (hrepeat do 1 unfold_mod; s); i; ss
     | eapply ISim.sim_fun_strong; try unfold_mod_fn; i; des; subst; ss
     ]
-  ]).
+  ]). *)
 
-Ltac iinit_simF := initialize_simF.
+(* Ltac iinit_simF := initialize_simF. *)
+Lemma wsim_HoareFun_src `{!crisG Γ Σ α β τ _S _I, !concG}
+    fsp msk fbd arg fl_src fl_tgt Ist RR r g ps pt st_src st_tgt itr_tgt :
+  (∀ N tid x varg, TID tid -∗
+    YIELD tid -∗
+    precond fsp (N, tid) x varg arg -∗
+    wsim fl_src fl_tgt Ist (↑N, ↑N) r g Any.t Any.t
+      (λ src tgt, TID tid ∗ YIELD tid ∗ winv (↑N, ↑N) ∗
+        ∃ ret, postcond fsp (N, tid) x src.2 ret ∗ RR (src.1, ret) tgt) true pt
+      (st_src, SB.sandbox msk (fbd N tid varg))
+      (st_tgt, itr_tgt)) ⊢
+  wsim fl_src fl_tgt Ist (∅, ∅) r g Any.t Any.t RR ps pt
+    (st_src, SB.sandbox msk (SModTr.HoareFun (Some fsp) fbd arg))
+    (st_tgt, itr_tgt).
+Proof.
+  iIntros "sim".
+  rewrite /SModTr.HoareFun.
+  norm_l. des_if; step_l; ss. destruct _q as [N tid].
+  steps_l. des_if; step_l; ss. rename _q into m.
+  steps_l. des_if; step_l; ss. rename _q into varg.
+  steps_l. des_if; step_l; ss.
+  iDestruct "ASM" as "[? [? W]]"; iApply wsim_fold; iFrame "W".
+  steps_l. des_if; step_l; ss. steps_l.
+  rewrite {2}(bind_ret_r_rev itr_tgt).
+  iPoseProof ("sim" with "[$] [$] [$]") as "sim".
+  iApply wsim_bind; iFrame "sim".
+  clear dependent st_src st_tgt.
+  iIntros (st_src r_s st_tgt r_t) "[? [? [W [%ret [Post RR]]]]]".
+  steps_l. des_ifs; steps_l; ss.
+  force_l ret. steps_l. des_ifs; steps_l; ss.
+  forces_l. iFrame. steps_l. des_ifs; steps_l; ss. force_l. iFrame "Post". step; ss.
+Qed.
+
+Ltac init_simF :=
+  rewrite /ISim.sim_fun; simpl_map; intros ??; eexists; split; first refl;
+  iIntros (arg st_src st_tgt) "IST"; iApply wsim_isim;
+  rewrite /SB.sandbox_body /=.
+
+Ltac iStartSim := init_simF; unfold_cris_defs; iApply wsim_HoareFun_src; eauto; ss.
