theories/simulations/msim/WTactics.v
@@ -1,6 +1,97 @@
 From iris.proofmode Require Import proofmode.
 Require Import Common Mod ltac2_lib.
-Require Import WSim TacticsCommon TacticsInit.
+Require Import WSim TacticsCommon.
+
+Ltac is_key_in k m :=
+  match m with
+  | {[ k := _ ]} => idtac
+  | <[ k := _ ]> _ => idtac
+  | <[ _ := _ ]> ?rest => is_key_in k rest
+  | union_with _ ?l ?r => first [ is_key_in k l | is_key_in k r ]
+  | _ => fail "Key not syntactically found"
+  end.
+
+Ltac solve_map_lookup_symbolic NODT :=
+  match goal with
+  | [ |- union_with ?f ?l ?r !! ?k = _ ] =>
+      tryif is_key_in k l 
+      then (
+        eapply lookup_union_with_l;
+        [eauto|eapply map_Forall_union_with in NODT as [NODT _]];
+        solve_map_lookup_symbolic NODT
+      )
+      else (
+        eapply lookup_union_with_r;
+        [eauto|eapply map_Forall_union_with in NODT as [_ NODT]];
+        solve_map_lookup_symbolic NODT
+      )
+  | [ |- <[ ?k' := ?v ]> ?m !! ?k = _ ] =>
+      (* Case: Insert *)
+      tryif unify k' k
+      then (rewrite lookup_insert; reflexivity)
+      else (
+        rewrite lookup_insert_ne; [|let Hc := fresh "" in intro Hc; inversion Hc; done];
+        solve_map_lookup_symbolic NODT
+      )
+  | [ |- {[ ?k' := ?v ]} !! ?k = _ ] =>
+      (* Case: Singleton *)
+      unify k' k; apply lookup_singleton
+  | |- ?A => 
+      (* idtac "Leaf reached or structure unknown";  *) fail
+  end.
+
+Ltac state_lookup_simpl NOD :=
+  let GOAL := fresh "GOAL" in
+  set (a := _ !! _); pattern a; subst a;
+  match goal with [|- ?G _] => set (GOAL := G) end;
+  eapply (eq_ind_r GOAL); [|solve_map_lookup_symbolic NOD];
+  rewrite /GOAL /=; clear GOAL.
+
+(* TODO : the complexity of this tactic is terrible - make it better *)
+Ltac state_insert_simpl NODT :=
+  let GOAL := fresh "GOAL" in
+  set (a := <[_:=_]> _); pattern a; subst a;
+  match goal with [|- ?G _] => set (GOAL := G) end;
+  eapply (eq_ind_r GOAL);
+  [|
+    match goal with
+    | [ |- <[?k:=?v]> (union_with ?f ?l ?r) = _ ] =>
+        tryif is_key_in k l
+        then (
+          etransitivity;
+          [ eapply insert_union_with_l';
+            [ eauto
+            | eapply map_Forall_union_with in NODT as [NODT _];
+              eexists; state_lookup_simpl NODT; reflexivity
+            ]
+          | eapply map_Forall_union_with in NODT as [NODT _]; 
+            state_insert_simpl NODT ]
+        )
+        else (
+          etransitivity;
+          [ eapply insert_union_with_r';
+            [ eauto
+            | eapply map_Forall_union_with in NODT as [_ NODT];
+              eexists; state_lookup_simpl NODT; reflexivity
+            ]
+          | eapply map_Forall_union_with in NODT as [_ NODT]; 
+            state_insert_simpl NODT ]
+        )
+    | [ |- <[?k:=_]>{[?k':=?v]} = _ ] => (* Case: Singleton *)
+        unify k' k; apply insert_singleton
+    | [ |- <[?k:=_]>(<[?k':=?v]>?m) = _ ] => (* Case: Insert *)
+        tryif unify k' k
+        then (rewrite insert_insert; reflexivity)
+        else (
+          rewrite insert_ne; [|let Hc := fresh "" in intro Hc; inversion Hc; done];
+          state_insert_simpl NODT
+        )
+    
+    | |- ?A => 
+        (* idtac "Leaf reached or structure unknown";  *) fail
+    end
+  ];
+  rewrite /GOAL //=; clear GOAL.
 
 Ltac _wstep_l :=
   match goal with
@@ -12,16 +103,6 @@ Ltac _wstep_l :=
       let name := fresh "_q" in iApply wsim_take_src; iIntros (name)
   | [ |- environments.envs_entails _ (wsim _ _ _ _ _ _ _ _ _ _ _ (_, trigger (Assume ?P) >>= _) _) ] =>
       unfold_pre_post_term P; iApply wsim_assume_src; iIntrosFresh "ASM"
-      (* first [
-        tcsearch constr:(WP P)
-          ltac:(fun c =>
-            iApply (wsim_assume_src_WP _ _ _ _ _ _ _ _ _ _ _ _ _ _ _ (i:=c)); simpl);
-        match goal with
-        | [ |- environments.envs_entails _ (?P' -∗ _)] =>
-          unfold_pre_post_term P'; iIntrosFresh "ASM"
-        end
-      | unfold_pre_post_term P; iApply wsim_assume_src; iIntrosFresh "ASM"
-      ] *)
   | [ |- environments.envs_entails _ (wsim _ _ _ _ _ _ _ _ _ _ _ (_, trigger (AssumeRes _) >>= _) _) ] =>
       iApply wsim_assume_res_src; iIntrosFresh "ASM"
   | [ |- environments.envs_entails _ (wsim _ _ _ _ _ _ _ _ _ _ _ (_, assume _ >>= _) _) ] =>
@@ -36,7 +117,6 @@ Ltac _wstep_l :=
       iApply wsim_unwrapU_src; iIntros (name) "%";
       match goal with [ H: ?x = Some _ |- _ ] => let G := fresh "G" in rename H into G; try rewrite -> G in * end
   end.
-
 Ltac wstep_l_core :=
   _wstep_l; try alist_find_simpl; s; des_pairs; s.
 
@@ -61,24 +141,17 @@ Ltac _wstep_r :=
   | [ |- environments.envs_entails _ (wsim _ _ _ _ _ _ _ _ _ _ _ _ (_, trigger (Choose _) >>= _) ) ] =>
       let name := fresh "_q" in iApply wsim_choose_tgt; iIntros (name)
   | [ |- environments.envs_entails _ (wsim _ _ _ _ _ _ _ _ _ _ _ _ (_, trigger (Guarantee ?P) >>= _) ) ] =>
-      (* first [
-        tcsearch constr:(WP P)
-          ltac:(fun c =>
-            iApply (wsim_guarantee_tgt_WP _ _ _ _ _ _ _ _ _ _ _ _ _ _ _ (i:=c)); simpl);
-        match goal with
-        | [ |- environments.envs_entails _ (?P' -∗ _)] =>
-            unfold_pre_post_term P'; iIntrosFresh "GRT"
-        end
-      | unfold_pre_post_term P; iApply wsim_guarantee_tgt; iIntrosFresh "GRT"
-      ] *)
       unfold_pre_post_term P; iApply wsim_guarantee_tgt; iIntrosFresh "GRT"
   | [ |- environments.envs_entails _ (wsim _ _ _ _ _ _ _ _ _ _ _ _ (_, guarantee _ >>= _)) ] =>
       let name := fresh "grt" in iApply wsim_guar_tgt; iIntros (name)
-  (* | [ |- environments.envs_entails _ (wsim _ _ _ _ _ _ _ _ _ _ _ _ (_, (SB.sandbox _ _ _ (trigger (SPut _ _))) >>= _)) ] =>
-      iApply wsim_nodup_tgt; iIntros (?); iApply wsim_sput_tgt_sandbox; [s; eauto|alist_upd_simpl]
-  | [ |- environments.envs_entails _ (wsim _ _ _ _ _ _ _ _ _ _ _ _ (_, (SB.sandbox _ _ _ (trigger (SGet _))) >>= _)) ] =>
-      let name := fresh "NODT" in
-      iApply wsim_nodup_tgt; iIntros (NODT); iApply wsim_sget_tgt_sandbox; [s; eauto|alist_find_simpl]; clear name *)
+  | [ |- environments.envs_entails _ (wsim _ _ _ _ _ _ _ _ _ _ _ _ (_, trigger (SGet _) >>= _)) ] =>
+      let NODT := fresh "NODT" in
+      iApply wsim_nodup_tgt; iIntros (NODT);
+      iApply wsim_sget_tgt; state_lookup_simpl NODT; clear NODT
+  | [ |- environments.envs_entails _ (wsim _ _ _ _ _ _ _ _ _ _ _ _ (_, trigger (SPut _ _) >>= _)) ] =>
+      let NODT := fresh "NODT" in
+      iApply wsim_nodup_tgt; iIntros (NODT);
+      iApply wsim_sput_tgt; state_insert_simpl NODT; clear NODT
   end.
 
 Ltac wstep_r_core :=
@@ -98,7 +171,7 @@ Ltac wsteps_r :=
 Ltac _wstep :=
   match goal with
   | [ |- environments.envs_entails _ (wsim _ _ _ _ _ _ _ _ _ _ _ (_, Ret _) (_, Ret _))] =>
-      iApply wsim_ret
+      iApply wsim_unfold; iIntros "?"; iApply wsim_ret; iFrame
   | [ |- environments.envs_entails _ (wsim _ _ _ _ _ _ _ _ _ _ _ (_, trigger (IO _ _) >>= _) (_, trigger (IO _ _) >>= _))] =>
       iApply wsim_io; iIntros "%"
   | [ |- environments.envs_entails _ (wsim _ _ _ _ _ _ _ _ _ _ _ (_, trigger GetTid >>= _) (_, trigger GetTid >>= _))] =>
@@ -106,7 +179,7 @@ Ltac _wstep :=
   end.
 
 Ltac wstep :=
-  norm with do 1 _wstep; s; des_pairs; s.
+  norm with do 1 _wstep.
 
 Ltac _wforce_l :=
   match goal with
@@ -207,13 +280,13 @@ Ltac wby_coind CIH :=
   iApply wsim_progress; iApply wsim_base; iIntrosFresh "I";
   iApply CIH.
 
-Ltac winit_simF :=
+(* Ltac winit_simF :=
   initialize_simF;
   iApply wsim_isim;
   try (
       iDestruct "IST" as "[% [W [TID IST]]]"; des; subst;
       iApply wsim_init_winv; iSplitL "W"; [et; fail|]; hss_copset;
-      hrepeat do 1 (unfold_mod; s)).
+      hrepeat do 1 (unfold_mod; s)). *)
 
 (** Special Tactics for RealUpdate **)
 
